theories/case_studies/generator_iterator.v
@@ -17,6 +17,7 @@ From haffel.lang Require Import haffel.
 From haffel.logic Require Import sem_def.
 From haffel.logic Require Import sem_env.
 From haffel.logic Require Import sem_sig.
+From haffel.logic Require Import sem_row.
 From haffel.logic Require Import sem_judgement.
 From haffel.logic Require Import sem_types.
 From haffel.logic Require Import copyable.
@@ -24,11 +25,11 @@ From haffel.logic Require Import sem_operators.
 From haffel.logic Require Import tactics.
 From haffel.logic Require Import compatibility.
 
-Definition yield := (λ: "x", perform: "x")%V.
+Definition yield := (λ: "x", perform: (effect "yield", "x"))%V.
 Definition generate :=
   (Λ: λ: "i", let: "cont" := ref (λ: <>, "i" <_> yield) in
       λ: <>, let: "comp" := "cont" <!- (λ: <>, #())  in
-             shallow-try: "comp" #() with
+              shallow-try-ls: "comp" #() handle "yield" with
                 effect λ: "x" "k", "cont" <- "k" ;; SOME "x"
              |  return λ: "x", NONE
              end
@@ -47,9 +48,9 @@ Section typing.
 
   Context `{!heapGS Σ}.
 
-  Definition yield_sig (τ : sem_ty Σ) := (μ∀TS: _, _, τ ⇒ () | OS)%S.
-  Definition yield_ty τ := τ -{ yield_sig τ }-> ().
-  Definition iter_ty τ := (∀S: θ, (τ -{ ¡ θ }-> ()) -{ ¡ θ }-∘ ())%T.
+  Definition yield_sig (τ : sem_ty Σ) : label * sem_sig Σ := ("yield", ∀S: _, τ ⇒ () | OS)%S.
+  Definition yield_ty τ := τ -{ (yield_sig τ ·: ⟨⟩) }-> ().
+  Definition iter_ty τ := (∀R: θ, (τ -{ ¡ θ }-> ()) -{ ¡ θ }-∘ ())%T.
   Definition generator_ty τ := (() → Option τ)%T.
   
   Lemma sem_typed_generate :
@@ -57,45 +58,40 @@ Section typing.
   Proof.
     iIntros "". iApply sem_typed_Tclosure. iIntros (α).
     rewrite -(app_nil_r []). iApply sem_typed_ufun; solve_sidecond. simpl.
-    set cont_ty := (() -{ yield_sig α }-∘ ()). 
-    iApply (sem_typed_let _ [] _ _ _ _ (Refᶜ cont_ty)); simpl; solve_sidecond. 
+    set cont_ty := (() -{ yield_sig α ·: ⟨⟩ }-∘ ()). 
+    iApply (sem_typed_let (Refᶜ cont_ty) _ _ _ []); simpl; solve_sidecond. 
     - iApply sem_typed_alloc_cpy.
       rewrite -(app_nil_r [("i", _)]).
       iApply sem_typed_afun; solve_sidecond. simpl.
-      iApply (sem_typed_app _ [("i", iter_ty α)] _ _ _ (yield_ty α)); solve_sidecond.
+      iApply (sem_typed_app (yield_ty α) _ _ _ [("i", iter_ty α)]); solve_sidecond.
       + iApply sem_typed_sub_nil.
         iApply sem_typed_sub_ty.
-        { iApply ty_le_aarr;[iApply sig_le_os| |iApply ty_le_refl]. 
-          iApply ty_le_uarr; try iApply ty_le_refl.
-          iApply sig_le_os_inv. }
-        iApply (sem_typed_SApp _ _ _ ⊥ _ (λ ρ, ( α -{ ¡ ρ }-> ()) -{ ¡ ρ }-∘ ())); solve_sidecond.
+        { iApply ty_le_aarr;[iApply row_le_os_elim| |iApply ty_le_refl]. 
+          rewrite /yield_ty. iApply ty_le_uarr; try iApply ty_le_refl.
+          iApply row_le_os_intro. }
+        iApply (sem_typed_RApp (λ ρ, ( α -{ ¡ ρ }-> ()) -{ ¡ ρ }-∘ ())); solve_sidecond.
         iApply sem_typed_var.
       + iApply sem_typed_frame. iApply sem_typed_sub_nil.
-        iApply sem_typed_val. iApply sem_typed_closure; first done.
-        simpl. iApply (sem_typed_perform_os _ _ _ () with "[]"). 
-        iApply sem_typed_sub_nil. iApply sem_typed_var.
+        iApply sem_typed_val. rewrite /yield /yield_ty. iApply sem_typed_closure; solve_sidecond.
+        simpl. iApply (sem_typed_perform_os () with "[]"). 
+        iApply sem_typed_var'.
     - set Γ₁ :=[("cont", Refᶜ cont_ty)]; rewrite -(app_nil_r Γ₁). 
       iApply sem_typed_ufun; solve_sidecond. simpl.
-      iApply (sem_typed_let _ [("cont", Refᶜ cont_ty)] _ _ _ _ cont_ty); solve_sidecond.
+      iApply (sem_typed_let cont_ty _ _ _ [("cont", Refᶜ cont_ty)]); solve_sidecond.
       + iApply sem_typed_contraction; solve_sidecond.
-        iApply sem_typed_replace_cpy.
-        { iApply sem_typed_sub_nil. iApply sem_typed_var. }
-        do 2 (iApply sem_typed_frame).
-        rewrite -(app_nil_r []).
+        iApply sem_typed_replace_cpy; first iApply sem_typed_var'.
+        do 2 (iApply sem_typed_frame). rewrite -(app_nil_r []).
         iApply sem_typed_afun; solve_sidecond.
-        simpl. iApply sem_typed_sub_nil. iApply sem_typed_unit.
+        simpl. iApply sem_typed_unit'.
       + rewrite app_singletons.
-        iApply (sem_typed_shallow_try_os OS
-                      [("comp", cont_ty)] [] [] [("cont", Refᶜ cont_ty)] 
-                      "x" "k" _ _ _ (λ _ _, α) (λ _ _, ()) () (Option α)); solve_sidecond.
-        * iApply sem_typed_app; first solve_sidecond; 
-          iApply sem_typed_sub_nil;
-            [iApply sem_typed_var|iApply sem_typed_unit]. 
+        iApply (sem_typed_shallow_try_os OS "yield" (λ _, α) (λ _, ()) () (Option α) ⊥ _ 
+                      [("comp", cont_ty)] [] [] [("cont", Refᶜ cont_ty)]); solve_sidecond.
+        { iApply row_le_refl. }
+        * iApply sem_typed_app; [iApply sem_typed_var'|iApply sem_typed_unit']. 
         * iIntros (?). do 2 iApply sem_typed_swap_third.
-          iApply (sem_typed_seq _ [("x", α)]).
+          iApply sem_typed_seq.
           { iApply sem_typed_store_cpy; iApply sem_typed_var. }
-          iApply sem_typed_some.
-          iApply sem_typed_var.
+          iApply sem_typed_some. iApply sem_typed_var.
         * simpl. do 2 iApply sem_typed_weaken.
           iApply sem_typed_none.
   Qed.
@@ -105,34 +101,29 @@ Section typing.
   Proof.
     iIntros. iApply sem_typed_closure; first done. rewrite /iter_ty /=.
     rewrite - {1}(app_nil_r [("g", _)]). 
-    iApply sem_typed_SLam; solve_sidecond. iIntros (θ).
+    iApply sem_typed_RLam; solve_sidecond. iIntros (θ).
     rewrite - {1}(app_nil_r [("g", _)]). 
     iApply sem_typed_sub_nil. 
     iApply sem_typed_afun; solve_sidecond. simpl.
     iApply sem_typed_app;
-      [|iApply sem_typed_sub_nil; iApply sem_typed_swap_second; iApply sem_typed_var].
+      [|iApply sem_typed_swap_second; iApply sem_typed_var'].
     rewrite - {1}((app_nil_r [("f", _)])). 
-    iApply sem_typed_sub_ty; [iApply ty_le_u2aarr|].
-    iApply sem_typed_sub_nil.
+    iApply sem_typed_sub_u2aarr. iApply sem_typed_sub_nil.
     iApply sem_typed_ufun; solve_sidecond. simpl.
     set Γ₂ := [("g", generator_ty τ); ("go", generator_ty τ -{ ¡ θ }-> () ); ("f", τ -{ ¡ θ }-> ())].
-    iApply (sem_typed_match_option _ Γ₂ _ _ _ _ _ (¡ θ)%S τ); solve_sidecond.
-    - iApply sem_typed_sub_nil. 
-      iApply sem_typed_app; solve_sidecond; last iApply sem_typed_unit.
+    iApply (sem_typed_match_option (¡ θ)%R τ _ _ Γ₂); solve_sidecond.
+    - iApply sem_typed_sub_nil.
+      iApply sem_typed_app; solve_sidecond; last iApply sem_typed_unit'.
       iApply sem_typed_contraction; solve_sidecond. 
-      iApply sem_typed_sub_nil. 
-      iApply sem_typed_sub_ty; [iApply ty_le_u2aarr|iApply sem_typed_var].
-    - iApply sem_typed_sub_nil. do 3 iApply sem_typed_weaken. iApply sem_typed_unit.
-    - iApply (sem_typed_seq _ [("g", generator_ty τ ); ("go", generator_ty τ -{ ¡ θ }-> ())]).
+      iApply sem_typed_sub_u2aarr. iApply sem_typed_var'.
+    - do 3 iApply sem_typed_weaken. iApply sem_typed_unit'.
+    - iApply sem_typed_seq.
       + iApply sem_typed_app.
-        { iApply sem_typed_sub_nil. iApply sem_typed_sub_ty; first iApply ty_le_u2aarr.
-          iApply sem_typed_var. }
-        iApply sem_typed_sub_nil. 
+        { iApply sem_typed_sub_u2aarr. iApply sem_typed_var'. }
         iApply sem_typed_swap_fourth. iApply sem_typed_swap_second.
-        iApply sem_typed_var.
-      + iApply sem_typed_app; [|iApply sem_typed_sub_nil; iApply sem_typed_var].
-        iApply sem_typed_sub_nil. iApply sem_typed_sub_ty; [iApply ty_le_u2aarr|].
-        iApply sem_typed_var.
+        iApply sem_typed_var'.
+      + iApply sem_typed_app; [|iApply sem_typed_var'].
+        iApply sem_typed_sub_u2aarr. iApply sem_typed_var'.
   Qed.
 
 End typing.
