theories/case_studies/state.v
@@ -17,6 +17,7 @@ From haffel.lang Require Import haffel.
 From haffel.logic Require Import sem_def.
 From haffel.logic Require Import sem_env.
 From haffel.logic Require Import sem_sig.
+From haffel.logic Require Import sem_row.
 From haffel.logic Require Import sem_types.
 From haffel.logic Require Import sem_judgement.
 From haffel.logic Require Import copyable.
@@ -24,8 +25,8 @@ From haffel.logic Require Import sem_operators.
 From haffel.logic Require Import compatibility.
 From haffel.logic Require Import tactics.
 
-Definition get : val := (λ: <>, performₘ: (InjL #()))%V.
-Definition put : val := (λ: "s", (performₘ: InjR "s") ;; #())%V.
+Definition get : val := (λ: <>, performₘ: (effect "get", #()))%V.
+Definition put : val := (λ: "s", (performₘ: (effect "put", "s")))%V.
 
 Definition fact : val :=
   (rec: "fact" "n" := if: #1 < "n" then put (get #() * "n");; "fact" ("n" - #1)
@@ -33,161 +34,135 @@ Definition fact : val :=
 
 Definition fact_ref : val :=
   (λ: "n", let: "store" := ref #1 in
-            deep-try: (fact "n") with
-              effect (λ: "x" "k",
-                match: "x" with 
-                  InjL <> => 
-                    (* get effect *)
-                    "k" (Load "store")
-                | InjR "s" =>
-                    (* put effect *)
-                    "store" <- "s" ;; "k" (Load "store") 
-                end)%E
-            | return (λ: "x", Load "store")%E end)%V.
+      deep-try-ls2: (fact "n") with
+          effect "get" => (λ: "x" "k", "k" (Load "store"))
+        | effect "put" => (λ: "x" "k", "store" <- "x" ;; "k" #())
+        | return (λ: "x", Load "store")
+      end)%V.
 
 Definition fact_st : val :=
-  (λ: "n", deep-try: (fact "n") with
-              effect (λ: "x" "k",
-                match: "x" with 
-                  InjL <> => 
-                    (* get effect *) 
-                    (λ: "s", "k" "s" "s")%E
-                | InjR "s" =>
-                    (* put effect *) 
-                    (λ: <>, "k" "s" "s")%E
-                end)%E
-            | return (λ: "x", (λ: "y", "y")%V)%E end #1)%V.
+  (λ: "n", 
+    (deep-try-ls2: (fact "n") with
+        effect "get" => (λ: "x" "k", (λ: "s", "k" "s" "s"))
+      | effect "put" => (λ: "x" "k", (λ: <>, "k" #() "x"))
+      | return (λ: "x", (λ: "y", "y"))
+      end #1))%V.
 
 Section typing.
 
   Context `{!heapGS Σ}.
 
-  Definition stsig : sem_sig Σ := (μ∀TS: _ , _, () + ℤ ⇒ ℤ | MS)%S.
+  Definition putsig : label * sem_sig Σ := ("put", ∀S: _, ℤ ⇒ () | MS)%S.  
+  Definition getsig : label * sem_sig Σ := ("get", ∀S: _, () ⇒ ℤ | MS)%S.
+  Definition st : sem_row Σ := (putsig ·: getsig ·: ⟨⟩)%R.
 
   Lemma get_typed :
-    ⊢ ⊨ᵥ get : (() -{ stsig }-> ℤ).
+    ⊢ ⊨ᵥ get : (() -{ st }-> ℤ).
   Proof.
     iIntros. iApply sem_typed_closure; solve_sidecond.
-    simpl. iApply (sem_typed_perform_ms _ _ _ () with "[] []"); first solve_copy.
-    simpl. iApply sem_typed_left_inj. 
-    iApply sem_typed_sub_nil. iApply sem_typed_unit.
+    simpl. rewrite /st. iApply sem_typed_sub_row.
+    { by iApply row_le_swap_second. }
+    iApply (sem_typed_perform_ms () with "[] []"); first solve_copy.
+    simpl. iApply sem_typed_unit'.
   Qed.
 
   Lemma put_typed :
-    ⊢ ⊨ᵥ put : (ℤ -{ stsig }-> ()).
+    ⊢ ⊨ᵥ put : (ℤ -{ st }-> ()).
   Proof.
     iIntros. iApply sem_typed_closure; solve_sidecond.
-    simpl. iApply (sem_typed_seq _ []);
-      last (iApply sem_typed_sub_nil; iApply sem_typed_unit).
-    iApply (sem_typed_perform_ms _ _ _ () with "[] []"); first solve_copy.
-    simpl. iApply sem_typed_right_inj. 
-    iApply sem_typed_sub_nil. iApply sem_typed_var.
+    iApply (sem_typed_perform_ms () with "[] []"); first solve_copy.
+    iApply sem_typed_var'.
   Qed.
 
+
   Lemma fact_typed :
-    ⊢ ⊨ᵥ fact : (ℤ -{ stsig }-> ()).
+    ⊢ ⊨ᵥ fact : (ℤ -{ st }-> ()).
   Proof.
     iIntros. iApply sem_typed_closure; solve_sidecond.
     set n := ("n", ℤ : sem_ty Σ).
-    set fact := ("fact", ℤ -{ stsig }-> () : sem_ty Σ).
+    set fact := ("fact", ℤ -{ st }-> () : sem_ty Σ).
     rewrite /= -/n -/fact.
-    iApply (sem_typed_if _ [n; fact]);
-      last (iApply sem_typed_sub_nil; 
-            do 2 iApply sem_typed_weaken;
-            iApply sem_typed_unit).
-    { iApply sem_typed_sub_nil. 
-      iApply sem_typed_contraction; solve_sidecond.
-      iApply sem_typed_bin_op; [constructor|iApply sem_typed_int|].
-      iApply sem_typed_var. }
-    iApply (sem_typed_seq _ [n;fact]).
+    iApply (sem_typed_if _ _ _ [n; fact]);
+      last (do 2 iApply sem_typed_weaken; iApply sem_typed_unit').
+    { iApply sem_typed_contraction; solve_sidecond.
+      iApply sem_typed_bin_op; [constructor|iApply sem_typed_int'|].
+      iApply sem_typed_var'. }
+    iApply (sem_typed_seq _ _ _ _ [n;fact]).
     - iApply sem_typed_contraction; solve_copy.
       iApply sem_typed_frame_ms; first solve_copy.
       iApply sem_typed_swap_second.
       iApply sem_typed_frame_ms; first solve_copy.
-      iApply (sem_typed_app_ms _ [] _ _ _ ℤ); solve_sidecond.
-      { iApply sem_typed_sub_nil. 
-        iApply sem_typed_sub_ty; [iApply ty_le_u2aarr|].
+      iApply (sem_typed_app_ms ℤ); solve_sidecond.
+      { iApply sem_typed_sub_u2aarr. iApply sem_typed_sub_nil.
         iApply sem_typed_val. iApply put_typed. }
       iApply sem_typed_bin_op; 
-        [constructor| |iApply sem_typed_sub_nil;iApply sem_typed_var].
-      iApply (sem_typed_app_ms _ _ _ _ _ ()); solve_sidecond; 
-        last (iApply sem_typed_sub_nil; iApply sem_typed_unit).
-      iApply sem_typed_sub_nil; 
-      iApply sem_typed_sub_ty; [iApply ty_le_u2aarr|].
+        [constructor| |iApply sem_typed_var'].
+      iApply (sem_typed_app_ms ()); solve_sidecond; 
+        last (iApply sem_typed_unit').
+      iApply sem_typed_sub_nil; iApply sem_typed_sub_u2aarr.
       iApply sem_typed_val. iApply get_typed. 
-    - iApply (sem_typed_app_ms _ [fact] _ _ _ ℤ); solve_copy;
-        [iApply sem_typed_sub_ty; [iApply ty_le_u2aarr|];
-         iApply sem_typed_sub_nil; iApply sem_typed_var|].
-      iApply sem_typed_sub_nil.
+    - iApply (sem_typed_app_ms ℤ); solve_copy; 
+        [iApply sem_typed_sub_u2aarr; iApply sem_typed_var'|].
       iApply sem_typed_bin_op; 
-        [constructor|iApply sem_typed_var|iApply sem_typed_int].
+        [constructor|iApply sem_typed_var'|iApply sem_typed_int'].
   Qed.
 
   Lemma fact_ref_typed :
     ⊢ ⊨ᵥ fact_ref : (ℤ → ℤ).
   Proof.
     iIntros. iApply sem_typed_closure; solve_sidecond.
-    simpl. iApply (sem_typed_let _ [("n", ℤ)]); solve_sidecond. 
+    simpl. iApply (sem_typed_let _ _ _ _ [("n", ℤ)]); solve_sidecond. 
     { iApply sem_typed_alloc_cpy. iApply sem_typed_int. }
-    iApply sem_typed_swap_second.
-    rewrite app_singletons.
-    set A : sem_sig Σ → sem_ty Σ → sem_ty Σ := (λ _ _, () + ℤ)%T.
-    set B : sem_sig Σ → sem_ty Σ → sem_ty Σ := (λ _ _, ℤ)%T.
-    iApply (sem_typed_deep_try_os MS _ [] _ _ "x" _ _ _ _ A B () _ ⊥ with "[] [] []"); solve_sidecond.
-    { rewrite /A /B -/stsig. 
-      iApply (sem_typed_app_ms _ [] _ _ _ ℤ); solve_copy; 
-      iApply sem_typed_sub_nil; last (iApply sem_typed_var).
-      iApply sem_typed_sub_ty; [iApply ty_le_u2aarr|].
-      iApply sem_typed_val. iApply fact_typed. }
-    - iIntros (?). rewrite /A /B.
-      iApply (sem_typed_match _ [("k", _); ("store", _)]); 
-        solve_sidecond; [iApply sem_typed_var| |]; simpl.
-        + iApply sem_typed_app; [iApply sem_typed_var|].
-        iApply (sem_typed_load_cpy _ _ _ _ ℤ); solve_sidecond.
-        iApply sem_typed_swap_second. 
-        iApply sem_typed_var.
-      + iApply sem_typed_swap_third. iApply sem_typed_contraction; solve_sidecond.
-        iApply sem_typed_swap_third.
-        iApply (sem_typed_seq _ [("store", _); ("k", _)]). 
-        { iApply sem_typed_store_cpy; iApply sem_typed_var. }
-        iApply sem_typed_app; [iApply sem_typed_var|].
-        iApply (sem_typed_load_cpy _ _ _ _ ℤ); solve_sidecond.
-        iApply sem_typed_var.
-    - simpl. iApply sem_typed_weaken. iApply sem_typed_load_cpy; solve_sidecond.
-      iApply sem_typed_var.
+    iApply sem_typed_swap_second. rewrite app_singletons. 
+    iApply (sem_typed_deep_try_2_ms "get" "put" (λ _, ()) (λ _, ℤ) (λ _, ℤ) (λ _, ()) () ℤ ⊥ _ _ [] with "[] [] []"); solve_sidecond.
+    { iApply row_le_refl. }
+    - iApply sem_typed_sub_row; first by iApply row_le_swap_second.
+      iApply (sem_typed_app_ms ℤ); solve_copy; last iApply sem_typed_var'.
+      iApply sem_typed_sub_u2aarr. iApply sem_typed_sub_nil.
+      iApply sem_typed_val. iApply fact_typed.
+    - iIntros (?).  iApply sem_typed_weaken.
+      iApply sem_typed_swap_second. 
+      iApply (sem_typed_app_ms ℤ); solve_copy. 
+      { iApply sem_typed_sub_u2aarr. iApply sem_typed_var'. }
+      iApply (sem_typed_load_cpy ℤ); solve_sidecond.
+      iApply sem_typed_var'.
+    - iIntros (?).
+      iApply sem_typed_swap_third. iApply sem_typed_swap_second.
+      iApply (sem_typed_seq _ _ _ _  [("k", _)]).
+      { iApply sem_typed_store_cpy; iApply sem_typed_var'. }
+      iApply sem_typed_app; [iApply sem_typed_sub_u2aarr; iApply sem_typed_var'|].
+      iApply sem_typed_unit.
+    - simpl. iApply sem_typed_weaken. iApply (sem_typed_load_cpy ℤ); solve_sidecond.
+      iApply sem_typed_var'.
   Qed.
 
   Lemma fact_st_typed :
     ⊢ ⊨ᵥ fact_st : (ℤ → ℤ).
   Proof.
     iIntros. iApply sem_typed_closure; solve_sidecond.
-    simpl. iApply sem_typed_app; [|iApply sem_typed_int].
-    set A : sem_sig Σ → sem_ty Σ → sem_ty Σ := (λ _ _, () + ℤ)%T.
-    set B : sem_sig Σ → sem_ty Σ → sem_ty Σ := (λ _ _, ℤ)%T.
+    simpl. iApply (sem_typed_app_ms ℤ); solve_copy; last iApply sem_typed_int.
     rewrite - {1} (app_nil_r [("n", ℤ)]).
-    iApply (sem_typed_deep_try_os MS _ [] _ _ _ _ _ _ _ A B); solve_sidecond.
-    { rewrite /A /B -/stsig. 
-      iApply (sem_typed_app_ms _ _ _ _ _ ℤ); solve_copy; 
-      iApply sem_typed_sub_nil; last iApply sem_typed_var.
-      iApply sem_typed_sub_ty; [iApply ty_le_u2aarr|].
-      iApply sem_typed_val. iApply fact_typed. }
-    - iIntros (?). rewrite /A /B.
-      iApply (sem_typed_match _ [("k", _)]); 
-        solve_sidecond; [iApply sem_typed_var| |]; simpl.
-      + rewrite - {1} (app_nil_r [("k", _)]).
-        iApply sem_typed_afun; solve_sidecond. simpl.
-        iApply sem_typed_contraction; solve_sidecond.
-        do 2 (iApply sem_typed_app; [|iApply sem_typed_var]).
-        iApply sem_typed_var.
-      + rewrite - {1} (app_nil_r [("s", _); ("k", _)]).
-        iApply sem_typed_afun; solve_sidecond. simpl.
-        iApply sem_typed_contraction; solve_sidecond.
-        do 2 (iApply sem_typed_app; [|iApply sem_typed_var]).
-        iApply sem_typed_var.
+    iApply (sem_typed_deep_try_2_ms "get" "put" (λ _, ()) (λ _, ℤ) (λ _, ℤ) (λ _, ()) () _ _ _ _ []); solve_sidecond.
+    { iApply row_le_refl. }
+    - iApply sem_typed_sub_row; first by iApply row_le_swap_second.
+      iApply (sem_typed_app_ms ℤ); solve_copy; last iApply sem_typed_var'.
+      iApply sem_typed_sub_u2aarr. iApply sem_typed_sub_nil.
+      iApply sem_typed_val. iApply fact_typed.
+    - iIntros (?). iApply sem_typed_weaken.
+      rewrite - {1} (app_nil_r [("k", _)]).
+      iApply sem_typed_afun; solve_sidecond. simpl.
+      iApply (sem_typed_contraction _ _ _ _ _ ℤ); solve_sidecond.
+      do 2 (iApply (sem_typed_app_ms ℤ); solve_copy; last iApply sem_typed_var').
+      iApply sem_typed_sub_u2aarr. iApply sem_typed_var.
+    - iIntros (?).
+      rewrite - (app_nil_r [("x", _); ("k", _)]).
+      iApply sem_typed_afun; solve_sidecond. simpl.
+      iApply (sem_typed_app_ms ℤ); solve_copy; last iApply sem_typed_var.
+      iApply (sem_typed_app_ms ()); solve_copy; last iApply sem_typed_unit.
+      iApply sem_typed_sub_u2aarr. iApply sem_typed_var.
     - simpl. iApply sem_typed_weaken.
-      iApply sem_typed_sub_ty; [iApply ty_le_u2aarr|].
-      iApply sem_typed_val. iApply sem_typed_closure; solve_sidecond.
-      simpl. iApply sem_typed_var.
+      rewrite - (app_nil_r []).
+      iApply sem_typed_afun; solve_sidecond. iApply sem_typed_var.
   Qed.
 
 End typing.
